ebpf/Asm.v
@@ -111,10 +111,15 @@ Inductive cmpOp : Type :=
   | LE: signedness -> cmpOp. (**r e1 <= e2 *)
 
 Inductive sizeOp : Type :=
-  | Byte        (**r 1 byte *)
-  | HalfWord    (**r 2 bytes *)
-  | Word        (**r 4 bytes *)
-  | SignedWord. (**r 4 bytes (signed) *)
+  (** 32 bits *)
+| Byte        (**r 1 byte *)
+| HalfWord    (**r 2 bytes *)
+| Word        (**r 4 bytes *)
+| WordAny     (**r 4 bytes *)
+  (** 64 bits *)
+| SignedWord (**r 4 bytes (signed) *)
+| DBWord     (**r 8 bytes *)
+| DBWordAny.  (**r 8 bytes *)
 
 Inductive instruction : Type :=
   | Pload : sizeOp -> ireg -> ireg -> off -> instruction        (**r dereference load *)
@@ -289,22 +294,60 @@ Definition eval_cmp (op: cmpOp) (rs: regset) (m: mem) (r: ireg) (ri: ireg+imm) :
 
 (** Auxiliaries for memory accesses *)
 
-Definition size_to_memory_chunk (size: sizeOp) : memory_chunk :=
+(*Definition size_to_memory_chunk (size: sizeOp) : memory_chunk :=
   match size with
   | Byte => Mint8unsigned
   | HalfWord => Mint16unsigned
   | Word => Many32
   | SignedWord => Mint32
   end.
+ *)
+
+Definition load (k: sizeOp) (addr:val) (m:mem) :=
+  match k with
+  | Byte => Mem.loadv Mint8unsigned m addr
+  | HalfWord => Mem.loadv Mint16unsigned m addr
+  | Word     => Mem.loadv Mint32 m addr
+  | WordAny  => Mem.loadv Many32 m addr
+  | SignedWord => if Archi.ptr64
+                  then match Mem.loadv Mint32 m addr with
+                       | None => None
+                       | Some v => Some (Val.longofint v)
+                       end
+                  else None
+  | DBWord     => if Archi.ptr64 then Mem.loadv Mint64 m addr else None
+  | DBWordAny  => if Archi.ptr64 then Mem.loadv Many64 m addr else None
+  end.
 
 Definition exec_load (k: sizeOp) (r:ireg) (r':ireg) (o:Ptrofs.int) (rs: regset) (m:mem) :=
-  match Mem.loadv (size_to_memory_chunk k) m (Val.offset_ptr rs#r' o) with
+  match load k (Val.offset_ptr rs#r' o) m with
   | None => Stuck
   | Some v => Next (nextinstr (rs#r <- v)) m
   end.
 
+
+Definition cast_long_int (v:val) : val :=
+  match v with
+  | Vlong l => Vint (Int.repr (Int64.unsigned l))
+  | _       => Vundef
+  end.
+
+
+
+Definition store (k: sizeOp) (addr:val) (v:val) (m:mem) :=
+  match k with
+  | Byte => Mem.storev Mint8unsigned m addr v
+  | HalfWord => Mem.storev Mint16unsigned m addr v
+  | Word     => Mem.storev Mint32 m addr v
+  | WordAny  => Mem.storev Many32 m addr v
+  | SignedWord => if Archi.ptr64 then Mem.storev Mint32 m addr (cast_long_int v) else None
+  | DBWord     => if Archi.ptr64 then Mem.storev Mint64 m addr v else None
+  | DBWordAny  => if Archi.ptr64 then Mem.storev Many64 m addr v else None
+  end.
+
+
 Definition exec_store (k: sizeOp) (r:ireg) (ri:ireg+imm) (o:Ptrofs.int) (rs: regset) (m:mem) :=
-  match Mem.storev (size_to_memory_chunk k) m (Val.offset_ptr rs#r o) (eval_reg_imm rs ri) with
+  match store  k (Val.offset_ptr rs#r o) (eval_reg_imm rs ri) m with
   | None => Stuck
   | Some m' => Next (nextinstr rs) m'
   end.
