ebpf/Asmgenproof1.v
@@ -305,13 +305,14 @@ Proof.
   unfold stack_load in LOAD; ArgsInv.
   econstructor. split.
   - apply exec_straight_one. simpl; unfold exec_load.
-    + assert (H: Mem.loadv (size_to_memory_chunk x0) m (Val.offset_ptr (rs R10) ofs) = Some v). {
-        unfold chunk_of_type in TR.
-        unfold size_to_memory_chunk.
-        destruct ty, x0; try discriminate; auto.
-      }
-      rewrite H.
-      reflexivity.
+    +
+      unfold load, transl_typ in *.
+      destruct Archi.ptr64 eqn:A.
+      *
+        destruct ty; simpl in *; inv EQ1;
+        rewrite TR; reflexivity.
+      *  destruct ty; simpl in *; inv EQ1;
+        rewrite TR; reflexivity.
     + Simpl.
   - split; intros; Simpl.
 Qed.
@@ -328,39 +329,140 @@ Proof.
   unfold stack_store in STORE; ArgsInv.
   econstructor. split.
   - apply exec_straight_one. simpl; unfold exec_store.
-    + assert (H: Mem.storev (size_to_memory_chunk x0) m (Val.offset_ptr (rs R10) ofs) (rs x) = Some m'). {
-        unfold chunk_of_type in TR.
-        unfold size_to_memory_chunk.
-        destruct ty, x0; try discriminate; auto.
-      }
-      simpl.
-      rewrite H.
-      reflexivity.
+    + unfold store, transl_typ in *.
+      destruct Archi.ptr64 eqn:A.
+      *
+        destruct ty; simpl in *; inv EQ1;
+        rewrite TR; reflexivity.
+      *  destruct ty; simpl in *; inv EQ1;
+        rewrite TR; reflexivity.
     + Simpl.
   - intros; Simpl.
 Qed.
 
-Lemma transl_load_common_correct:
-  forall chunk k i op (x x0: ireg) (rs: regset) m a v,
+Lemma transl_load_indexed_correct:
+  forall chunk k i  (x x0: ireg) (rs: regset) m a v kl,
   Val.offset_ptr (rs x0) i = a ->
   Mem.loadv chunk m a = Some v ->
-  transl_memory_access chunk = OK op ->
+  transl_load_indexed chunk x x0 i k = OK kl ->
   exists rs',
-     exec_straight ge fn (Pload op x x0 i :: k) rs m k rs' m
+     exec_straight ge fn kl rs m k rs' m
   /\ rs'#x = v
   /\ forall r, r <> PC -> r <> x -> rs'#r = rs#r.
 Proof.
-  intros until v. intros EV LOAD TR.
-  econstructor. split.
-  - apply exec_straight_one; simpl; unfold exec_load.
-    + assert (H: Mem.loadv (size_to_memory_chunk op) m a = Some v). {
-        unfold transl_memory_access in TR.
-        destruct chunk, op; try discriminate; auto.
-      }
-      rewrite EV, H.
-      reflexivity.
-    + Simpl.
-  - split; intros; Simpl.
+  intros until v. intros KL EV LOAD TR.
+  unfold transl_load_indexed in TR.
+  destruct a; try discriminate.
+  unfold Mem.loadv in LOAD.
+  destruct chunk.
+  + (* Mint8signed *)
+    inv TR.
+    rewrite Mem.load_int8_signed_unsigned in LOAD.
+    destruct (Mem.load Mint8unsigned m b (Ptrofs.unsigned i0))eqn:ML; try discriminate.
+    simpl in LOAD. inv LOAD.
+    econstructor. split.
+    eapply exec_straight_three; simpl; unfold exec_load,load; try reflexivity.
+    unfold Mem.loadv. rewrite EV. rewrite ML.
+    reflexivity.
+    reflexivity.
+    split.
+    * Simpl.
+      destruct v0 ; simpl; auto.
+      change (Int.ltu (Int.repr 24) Int.iwordsize) with true.
+      simpl. change (Int.ltu (Int.repr 24) Int.iwordsize) with true.
+      simpl. rewrite Int.sign_ext_shr_shl. reflexivity.
+      change Int.zwordsize with 32. lia.
+    * Simpl.
+      intros.
+      Simpl.
+  + (* Mint8unsigned *)
+    inv TR.
+    econstructor. split.
+    eapply exec_straight_one; simpl; unfold exec_load,load; try reflexivity.
+    unfold Mem.loadv. rewrite EV. rewrite LOAD.
+    reflexivity.
+    reflexivity.
+    split.
+    * Simpl.
+    * intros.
+      Simpl.
+  + (* Mint16signed *)
+    inv TR.
+    rewrite Mem.load_int16_signed_unsigned in LOAD.
+    destruct (Mem.load Mint16unsigned m b (Ptrofs.unsigned i0))eqn:ML; try discriminate.
+    simpl in LOAD. inv LOAD.
+    econstructor. split.
+    eapply exec_straight_three; simpl; unfold exec_load,load; try reflexivity.
+    unfold Mem.loadv. rewrite EV. rewrite ML.
+    reflexivity.
+    reflexivity.
+    split.
+    * Simpl.
+      destruct v0 ; simpl; auto.
+      change (Int.ltu (Int.repr 16) Int.iwordsize) with true.
+      simpl. change (Int.ltu (Int.repr 16) Int.iwordsize) with true.
+      simpl. rewrite Int.sign_ext_shr_shl. reflexivity.
+      change Int.zwordsize with 32. lia.
+    * intros. Simpl.
+  + (* Mint16unsigned *)
+    inv TR.
+    econstructor. split.
+    eapply exec_straight_one; simpl; unfold exec_load,load; try reflexivity.
+    unfold Mem.loadv. rewrite EV. rewrite LOAD.
+    reflexivity.
+    reflexivity.
+    split.
+    * Simpl.
+    * intros.
+      Simpl.
+  + (* Mint32 *)
+    inv TR.
+    econstructor. split.
+    eapply exec_straight_one; simpl; unfold exec_load,load; try reflexivity.
+    unfold Mem.loadv. rewrite EV. rewrite LOAD.
+    reflexivity.
+    reflexivity.
+    split.
+    * Simpl.
+    * intros.
+      Simpl.
+  + destruct Archi.ptr64 eqn:A;[| discriminate].
+    (* Mint64 *)
+    inv TR.
+    econstructor. split.
+    eapply exec_straight_one; simpl; unfold exec_load,load; try reflexivity.
+    unfold Mem.loadv. rewrite EV. rewrite LOAD. rewrite A.
+    reflexivity.
+    reflexivity.
+    split.
+    * Simpl.
+    * intros.
+      Simpl.
+  + (* Mfloat32 *) discriminate.
+  + (* Mfloat64 *) discriminate.
+  + (* Many32 *)
+    inv TR.
+    econstructor. split.
+    eapply exec_straight_one; simpl; unfold exec_load,load; try reflexivity.
+    unfold Mem.loadv. rewrite EV. rewrite LOAD.
+    reflexivity.
+    reflexivity.
+    split.
+    * Simpl.
+    * intros.
+      Simpl.
+  + (* Many64 *)
+    destruct Archi.ptr64 eqn:A;[|discriminate].
+    inv TR.
+    econstructor. split.
+    eapply exec_straight_one; simpl; unfold exec_load,load; try reflexivity.
+    unfold Mem.loadv. rewrite EV. rewrite A.  rewrite LOAD.
+    reflexivity.
+    reflexivity.
+    split.
+    * Simpl.
+    * intros.
+      Simpl.
 Qed.
 
 Lemma transl_load_correct:
@@ -375,35 +477,91 @@ Lemma transl_load_correct:
 Proof.
   intros until v; intros TR EV LOAD.
   destruct addr, args; simpl in TR; ArgsInv.
-  - unfold transl_memory_access in EQ0.
-    inversion EV.
-    destruct chunk; try discriminate; eapply transl_load_common_correct; eauto.
-  - unfold transl_memory_access in EQ1.
-    inversion EV.
-    destruct chunk; try discriminate; eapply transl_load_common_correct; eauto.
+  - exploit transl_load_indexed_correct; eauto.
+    congruence.
+  - exploit transl_load_indexed_correct; eauto.
+    congruence.
 Qed.
 
 Lemma transl_store_common_correct:
-  forall chunk k i op (x x0: ireg) (rs: regset) m m' a,
+  forall chunk k i k' (x x0: ireg) (rs: regset) m m' a,
   Val.offset_ptr (rs x0) i = a ->
   Mem.storev chunk m a (rs x) = Some m' ->
-  transl_memory_access chunk = OK op ->
+  transl_store_indexed chunk x0 i x k = OK k' ->
   exists rs',
-     exec_straight ge fn (Pstore op x0 (inl x) i :: k) rs m k rs' m'
+     exec_straight ge fn k' rs m k rs' m'
   /\ forall r, r <> PC -> rs'#r = rs#r.
 Proof.
   intros until a. intros EV STORE TR.
-  econstructor. split.
-  - apply exec_straight_one; simpl; unfold exec_store.
-    + assert (H: Mem.storev (size_to_memory_chunk op) m a (rs x) = Some m'). {
-        unfold transl_memory_access in TR.
-        destruct chunk, op; try discriminate; auto.
-      }
-      simpl.
-      rewrite EV, H.
-      reflexivity.
-    + Simpl.
-  - intros; Simpl.
+  destruct chunk; simpl in TR.
+  - (* Mint8signed *)
+    inv TR.
+    econstructor. split.
+    apply exec_straight_one; simpl; unfold exec_store,store.
+    destruct (Val.offset_ptr (rs x0) i); try discriminate.
+    simpl in STORE.
+    rewrite Mem.store_signed_unsigned_8 in STORE.
+    simpl.
+    rewrite STORE. reflexivity.
+    reflexivity.
+    intros. Simplif.
+  - (* Mint8unsigned *)
+    inv TR.
+    econstructor. split.
+    apply exec_straight_one; simpl; unfold exec_store,store,eval_reg_imm.
+    rewrite STORE. reflexivity.
+    reflexivity.
+    intros. Simplif.
+  - (* Mint16signed *)
+    inv TR.
+    econstructor. split.
+    apply exec_straight_one; simpl; unfold exec_store,store.
+    destruct (Val.offset_ptr (rs x0) i); try discriminate.
+    simpl in STORE.
+    rewrite Mem.store_signed_unsigned_16 in STORE.
+    simpl.
+    rewrite STORE. reflexivity.
+    reflexivity.
+    intros. Simplif.
+  -
+    inv TR.
+    econstructor. split.
+    apply exec_straight_one; simpl; unfold exec_store,store,eval_reg_imm.
+    rewrite STORE. reflexivity.
+    reflexivity.
+    intros. Simplif.
+  -     inv TR.
+    econstructor. split.
+    apply exec_straight_one; simpl; unfold exec_store,store,eval_reg_imm.
+    rewrite STORE. reflexivity.
+    reflexivity.
+    intros. Simplif.
+  -
+    destruct Archi.ptr64 eqn:ARCHI;[|discriminate].
+    inv TR.
+    econstructor. split.
+    apply exec_straight_one; simpl; unfold exec_store,store,eval_reg_imm.
+    rewrite ARCHI.
+    rewrite STORE. reflexivity.
+    reflexivity.
+    intros. Simplif.
+  - discriminate.
+  - discriminate.
+  -
+    inv TR.
+    econstructor. split.
+    apply exec_straight_one; simpl; unfold exec_store,store,eval_reg_imm.
+    rewrite STORE. reflexivity.
+    reflexivity.
+    intros. Simplif.
+  -
+    destruct Archi.ptr64 eqn:ARCHI; [|discriminate].
+    inv TR.
+    econstructor. split.
+    apply exec_straight_one; simpl; unfold exec_store,store,eval_reg_imm.
+    rewrite STORE. rewrite ARCHI. reflexivity.
+    reflexivity.
+    intros. Simplif.
 Qed.
 
 Lemma transl_store_correct:
@@ -417,13 +575,10 @@ Lemma transl_store_correct:
 Proof.
   intros until m'; intros TR EV STORE.
   destruct addr, args; simpl in TR; ArgsInv.
-  - unfold transl_memory_access in EQ0.
-    inversion EV.
-    destruct chunk; try discriminate; eapply transl_store_common_correct; eauto.
-
-  - unfold transl_memory_access in EQ1.
-    inversion EV.
-    destruct chunk; try discriminate; eapply transl_store_common_correct; eauto.
+  - exploit transl_store_common_correct;eauto.
+    congruence.
+  - exploit transl_store_common_correct;eauto.
+    congruence.
 Qed.
 
 End CONSTRUCTORS.
